\begin{align}
\frac{dGPe_{+}x(t)}{dt} =& \frac{ - 2 \mathrm{GPe_{+}x}\left( t \right)}{GPe_+\tau} + \mathrm{GPe_{+}y}\left( t \right) \\
\frac{dGPe_{+}y(t)}{dt} =& \frac{GPe_{+}H \left(  - GPe_+\lambda + \frac{2 GPe_+\lambda}{1 + e^{ - GPe_{+}r \mathrm{GPe_{+}jcn}\left( t \right)}} \right)}{GPe_+\tau} + \frac{ - \mathrm{GPe_{+}x}\left( t \right)}{GPe_+\tau^{2}} \\
\frac{dSTN_{+}x(t)}{dt} =& \frac{ - 2 \mathrm{STN_{+}x}\left( t \right)}{STN_+\tau} + \mathrm{STN_{+}y}\left( t \right) \\
\frac{dSTN_{+}y(t)}{dt} =& \frac{STN_{+}H \left(  - STN_+\lambda + \frac{2 STN_+\lambda}{1 + e^{ - STN_{+}r \mathrm{STN_{+}jcn}\left( t \right)}} \right)}{STN_+\tau} + \frac{ - \mathrm{STN_{+}x}\left( t \right)}{STN_+\tau^{2}} \\
\frac{dGPi_{+}x(t)}{dt} =& \frac{ - 2 \mathrm{GPi_{+}x}\left( t \right)}{GPi_+\tau} + \mathrm{GPi_{+}y}\left( t \right) \\
\frac{dGPi_{+}y(t)}{dt} =& \frac{ - \mathrm{GPi_{+}x}\left( t \right)}{GPi_+\tau^{2}} + \frac{GPi_{+}H \left(  - GPi_+\lambda + \frac{2 GPi_+\lambda}{1 + e^{ - GPi_{+}r \mathrm{GPi_{+}jcn}\left( t \right)}} \right)}{GPi_+\tau} \\
\frac{dTh_{+}x(t)}{dt} =& \frac{ - 2 \mathrm{Th_{+}x}\left( t \right)}{Th_+\tau} + \mathrm{Th_{+}y}\left( t \right) \\
\frac{dTh_{+}y(t)}{dt} =& \frac{Th_{+}H \left(  - Th_+\lambda + \frac{2 Th_+\lambda}{1 + e^{ - Th_{+}r \mathrm{Th_{+}jcn}\left( t \right)}} \right)}{Th_+\tau} + \frac{ - \mathrm{Th_{+}x}\left( t \right)}{Th_+\tau^{2}} \\
\frac{dEI_{+}x(t)}{dt} =& \frac{ - 2 \mathrm{EI_{+}x}\left( t \right)}{EI_+\tau} + \mathrm{EI_{+}y}\left( t \right) \\
\frac{dEI_{+}y(t)}{dt} =& \frac{EI_{+}H \left(  - EI_+\lambda + \frac{2 EI_+\lambda}{1 + e^{ - EI_{+}r \mathrm{EI_{+}jcn}\left( t \right)}} \right)}{EI_+\tau} + \frac{ - \mathrm{EI_{+}x}\left( t \right)}{EI_+\tau^{2}} \\
\frac{dPY_{+}x(t)}{dt} =& \frac{ - 2 \mathrm{PY_{+}x}\left( t \right)}{PY_+\tau} + \mathrm{PY_{+}y}\left( t \right) \\
\frac{dPY_{+}y(t)}{dt} =& \frac{ - \mathrm{PY_{+}x}\left( t \right)}{PY_+\tau^{2}} + \frac{PY_{+}H \left(  - PY_+\lambda + \frac{2 PY_+\lambda}{1 + e^{ - PY_{+}r \mathrm{PY_{+}jcn}\left( t \right)}} \right)}{PY_+\tau} \\
\frac{dII_{+}x(t)}{dt} =& \frac{ - 2 \mathrm{II_{+}x}\left( t \right)}{II_+\tau} + \mathrm{II_{+}y}\left( t \right) \\
\frac{dII_{+}y(t)}{dt} =& \frac{ - \mathrm{II_{+}x}\left( t \right)}{II_+\tau^{2}} + \frac{II_{+}H \left(  - II_+\lambda + \frac{2 II_+\lambda}{1 + e^{ - II_{+}r \mathrm{II_{+}jcn}\left( t \right)}} \right)}{II_+\tau}
\end{align}
